\documentclass{article}
\usepackage[utf8]{inputenc}
\usepackage{natbib}
\usepackage{graphicx}
% \usepackage{tikz-cd}
\usepackage{tikz}
\usetikzlibrary{cd}
\usepackage{amsmath}
\usepackage{amssymb}
\usepackage{yfonts}
\usepackage{hyperref}
\usepackage{amsthm}
\usepackage{stmaryrd}
\usepackage{mathtools}
% \usepackage{floatrow}
\usepackage{subcaption}

\usepackage{geometry}
\geometry{
 a4paper,
 total={170mm,257mm},
 left=35mm,
 right=35mm,
 top=20mm,
 }

\hypersetup{
    colorlinks=true,
    linkcolor=blue,
    filecolor=magenta,      
    urlcolor=cyan,
}

\urlstyle{same}
%\newcommand{\goth}[1]{\text{\textgoth{#1}}

\newtheorem{theorem}{Step}

\title{Isomorphisms in Claim 1}

\begin{document}

\maketitle

\textbf{Isomorphism 1 to 2}

\[
  A_\textgoth{p} \otimes_A B/\textgoth{p}B \cong (B/\textgoth{p}B)_\textgoth{p}
\]

\begin{theorem}
How is $A_\textgoth{p} \otimes B/\textgoth{p}B$ a $B$-algebra?
\end{theorem}


We need a ring structure and a homomorphism from $B$. The first is defined in [ItCA] TENSOR PRODUCT OF ALGEBRAS pp 30-31.
\[
    \left( \frac{a}{s} \otimes (b + \textgoth{p}B) \right) \left( \frac{a'}{s'} \otimes (b' + \textgoth{p}B) \right) = \frac{aa'}{ss'} \otimes (bb' + \textgoth{p}B)
\]
but first the $B/\textgoth{p}B$has to be an algebra. That is, to be a ring. We have this in Facts, $\textgoth{p}B = \textgoth{p}^e$, an ideal of $B$ that does not have to be prime, still, $B/\textgoth{p}B$ is a ring.

The $B/\textgoth{p}B$ is a ring and a $B$-module. How is it a $B$-algebra? A homomorphism of rings? One proposition
\[
B \longrightarrow B/\textgoth{p}B
\]
\[
b \mapsto b + \textgoth{p}
\]

In the tensor product of algebras, $A \xrightarrow{f} B$, $A \xrightarrow{g} C$, the mapping from $A$ is $a \mapsto f(a) \otimes g(a)$, here the mapping from $B$ to $A_\textgoth{p} \otimes_A B/\textgoth{p}B$ is
\[
 b \mapsto \frac{b}{1} \otimes (b + \textgoth{p}B
\]
But are they both, the tensorands, $B$-algebras?

\vspace{10px}

What is $(B/\textgoth{p}B)_\textgoth{p}$? \\
$\textgoth{p}B$ is an ideal of $B$ . \\
$B/\textgoth{p}B$ is a ring and an $A$-module. \\
We can take the $(B/\textgoth{p}B)_\textgoth{p}$ $A\textgoth{p}$-module.

What a ring structure do we have on $(B/\textgoth{p}B)_\textgoth{p}$? General element is $(b + \textgoth{p}B)/s$. The obvious proposition is
\[
  \frac{b + \textgoth{p}B}{s} \cdot \frac{b' + \textgoth{p}B}{s'} = \frac{bb' + \textgoth{p}B}{ss'}
\]

Well-definition. Show that if
\[
\frac{b_1 + \textgoth{p}B}{s_1} = \frac{b_2 + \textgoth{p}B}{s_2}, \quad
\frac{b'_1 + \textgoth{p}B}{s'_!} = \frac{b'_2 + \textgoth{p}B}{s'_2} \tag{1}\label{eq:first}
\]
then
\[
\frac{b_1 b'_1 + \textgoth{p}B}{s_1 s'_1} = \frac{b_2 b'_2 + \textgoth{p}B}{s_2 s'_2} 
\tag{2}\label{eq:second}
\]
that is,
\[
v s_2 s_2' b_1 b_1' - v s_1 s_1' b_2 b_2' \in \textgoth{p}B
\tag{3}\label{eq:third}
\]
The \eqref{eq:first} means
\[
u(s_2(b_1 + \textgoth{p}B) - s_1(b_2 + \textgoth{p}B)) = 0, 
\]
\[
u'(s_2'(b_1' + \textgoth{p}B) - s_1'(b_2' + \textgoth{p}B)) = 0
\]
That is,
\[
u s_2 b_1 - u s_1 b_2 \in \textgoth{p}B,
\]
\[
u' s_2' b_1' - u' s_1' b_2' \in \textgoth{p}B,
\]
Then
\[
\overline{u s_2 b_1} = \overline{u s_1 b_2}, \quad 
\overline{u' s_2' b_1'} = \overline{u' s_1' b_2'}
\]
\[
\overline{u s_2 b_1 u' s_2' b_1'} =
\overline{u s_1 b_2 u' s_1' b_2'}
\]
\[
u u' s_2 s_2' b_1 b_1' - u u' s_1 s_1' b_2 b_2' \in  \textgoth{p}B
\]
And it is enough to take $v = u u'$ in \eqref{eq:third}.

Is a localization $B_\textgoth{p}$ of an $A$-algebra $B$ in a prime ideal $\textgoth{p}$ of $A$ a $B$-algebra? It is an $A_\textgoth{p}$-module. As the multiplication we try
\[
\frac{b}{s} \cdot \frac{b'}{s'} = \frac{b b'}{s s'}
\]
Well-definition.
\[
\frac{b_1}{s_1} = \frac{b_2}{s_2}, \quad \frac{b_1'}{s_1'} = \frac{b_2'}{s_2'} 
\implies
\frac{b_1 b_1'}{s_1 s_1'} = \frac{b_2 b_2'}{s_2 s_2'} \ ?
\]
The left
\[
u(s_2 b_1 - s_1 b_2) = 0, \quad u'(s_2' b_1' - s_1' b_2') = 0
\]
\[
u s_2 b_1 = u s_1 b_2, \quad u' s_2' b_1' = u' s_1' b_2'
\]
The right
\[
v(s_2 s_2' b_1 b_1' - s_1 s_1' b_2 b_2') = 0
\]
\[
v s_2 s_2' b_1 b_1' = v s_1 s_1' b_2 b_2'
\]
Take $v = u u'$. \\
Distributivity over addition.
\[
\frac{b}{s} \left( \frac{b'}{s'} + \frac{b''}{s''} \right) = 
\frac{b}{s} \frac{s'' b' + s' b''}{s' s''} = \frac{s'' b b' + s' b b''}{s s' s''}
\]
\[
\frac{b}{s}\frac{b'}{s'} + \frac{b}{s}\frac{b''}{s''} = 
\frac{b b'}{s s'} + \frac{b b''}{s s''} = \frac{s s'' b b' + s s' b b''}{s^2 s' s''} =
\frac{s(s'' b b' + s' b b'')}{s^2 s' s''} = 
\frac{s'' b b'' + s' b b''}{s s' s''}
\]

We now use this fact to get the multiplication in the $A$-algebra $B/\textgoth{p}B$ localized at an ideal $\textgoth{p}$ of $A$, that is, $(B/\textgoth{p}B)_\textgoth{p}$.
\[
\frac{b + \textgoth{p}B}{s} \cdot \frac{b' + \textgoth{p}B}{s'} = 
\frac{(b + \textgoth{p}B)(b' + \textgoth{p}B)}{s s'} = 
\frac{b b' + \textgoth{p}B}{s s'}
\]
which is an easier way to define this multiplication, avoiding lots of calculations.

We now move to to a proposition of mutually reverse maps between 
\[
A_\textgoth{p} \otimes_A B/\textgoth{p}B \quad  \text{and} \quad
(B/\textgoth{p}B)_\textgoth{p}
\]
Both are $B$-algebras. And $B$-algebras' isomorphisms must be commutative with homomorphisms from $B$.

\begin{figure}[htb]
\centering
\begin{subfigure}[T]{0.4\textwidth}
\centering
\begin{tikzcd}
& A_\textgoth{p} \otimes_A B/\textgoth{p}B \arrow[dd]  \\
B \arrow[ur] \arrow[dr] \\
& (B/\textgoth{p}B)_\textgoth{p}
\end{tikzcd}
\end{subfigure}
\centering
\begin{subfigure}[T]{0.4\textwidth}
\centering
\begin{tikzcd}
& A_\textgoth{p} \otimes_A B/\textgoth{p}B \arrow[dd]  \\
B \arrow[ur] \arrow[dr] \\
& (B/\textgoth{p}B)_\textgoth{p}
\end{tikzcd}
\end{subfigure}
\end{figure}

\end{document}

