\documentclass{article}
\usepackage[utf8]{inputenc}
\usepackage{natbib}
\usepackage{graphicx}
\usepackage{tikz-cd}
\usepackage{tikz}
\usetikzlibrary{cd}
\usepackage{amsmath}
\usepackage{amssymb}
\usepackage{yfonts}
\usepackage{hyperref}
\usepackage{amsthm}
\usepackage{stmaryrd}
\usepackage{mathtools}
% \usepackage{floatrow}
\usepackage{subcaption}

\usepackage{geometry}
\geometry{
 a4paper,
 total={170mm,257mm},
 left=35mm,
 right=35mm,
 top=20mm,
 }

\hypersetup{
    colorlinks=true,
    linkcolor=blue,
    filecolor=magenta,      
    urlcolor=cyan,
}

\urlstyle{same}

%\newcommand{\goth}[1]{\text{\textgoth{#1}}
\newcommand{\mf}{\mathfrak}
\newcommand{\aaa}{\mf a}
\newcommand{\bbb}{\mf b}
\newcommand{\ppp}{\mf p}
\newcommand{\qqq}{\mf q}
\newcommand{\Spec}{\operatorname{Spec}}

\newtheorem{theorem}{Step}

\title{Isomorphisms 2 to 3 of Claim 1}

\begin{document}

\maketitle

\textbf{Fact}. The isomorphism 2 to 3.
\[
  (B/\textgoth{p}B)_\textgoth{p} \cong 
  B_\textgoth{p} / \textgoth{p}_\textgoth{p} B_\textgoth{p}
\]
We know $\textgoth{p}_\textgoth{p} = \textgoth{p}A_\textgoth{p}$ is the single maximal ideal of $A_\textgoth{p}$. The map
\[
(B/\textgoth{p}B)_\textgoth{p} \rightarrow B_\textgoth{p}/\textgoth{p}_\textgoth{p}B_\textgoth{p}
\]
\[
\frac{b + \textgoth{p}B}{s} \mapsto \frac{b}{s} + \textgoth{p}_\textgoth{p}B_\textgoth{p}
\tag{1}\label{eq:first}
\]
Well-definition.
\[
\frac{b + \textgoth{p}B}{s} = \frac{b' + \textgoth{p}B}{s'}
\xRightarrow{?}
\frac{b}{s} - \frac{b'}{s'} \in \textgoth{p}B
\]
The left side of the implication.
\[
u(s'(b + \textgoth{p}B) - s(b' + \textgoth{p}B)) = 0 + \textgoth{p}B
\]
\[
us'b - usb' \in \textgoth{p}B
\]
\[
us'b - usb' = \sum a_i b_i
\tag{2}\label{eq:second}
\]
The right side of the implication.
\[
\frac{s'b - sb'}{ss'} \in \textgoth{p}_\textgoth{p}B_\textgoth{p} = \textgoth{p}A_\textgoth{p}B
\]
\begin{align*}
\frac{s'b - sb'}{ss'} & = \sum \frac{a_i}{s_i}\frac{b_i}{t_i} \\
& = \sum \frac{a_ib_i}{s_it_i} \\
& = \sum \frac{a_ib_i}{s_i'} \\
& = \frac{1}{s''} \sum a_i''b_i
\tag{3}\label{eq:third}
\end{align*}
\[
v(s''(s'b - sb') - ss' \sum a_i'' b_i) = 0
\]
\[
vs''s'b - vs''sb' = \sum vss'a_i''b_i
\]
Multiplying the equation \eqref{eq:second} by $s's$,
\[
us'^2sb - us's^2b' = \sum s'sa_ib_i
\]
Take $v = 1$, $s'' = u s's$, $a_i'' = a_i$ in \eqref{eq:third}. Our map \eqref{eq:first} is well-defined.

\vspace{4mm}
Proposition of inverse.
\[
B_\textgoth{p}/\textgoth{p}_\textgoth{p}B_\textgoth{p} \rightarrow (B/\textgoth{p}B)_\textgoth{p}
\]
\[
\frac{b}{s} \mapsto \frac{b}{s} + \textgoth{p}_\textgoth{p}B_\textgoth{p} 
\]
Well-definition.
\[
\frac{b}{s} - \frac{b'}{s'} \in \textgoth{p}A_\textgoth{p}B_\textgoth{p}
\xRightarrow{?}
\frac{b + \textgoth{p}B}{s} = \frac{b' + \textgoth{p}B}{s'}
\]
The left side of the implication.
\[
\frac{s'b - sb'}{ss'} = \frac{1}{s''}\sum a_i b_i
\]
\[
u(s''(s'b - sb') - ss' \sum a_ib_i) = 0
\]
\[
us''s'b - us''sb' = \sum us'sa_ib_i
\]
The right side of the implication.
\[
v(s'(b + \textgoth{p}B) - s(b' + \textgoth{p}B) = 0 + \textgoth{p}B
\]
\[
vs'b - vsb' \in \textgoth{p}B
\]
\[
vs'b - vsb' = \sum a_i'b_i'
\]
Take $v = us''$, $a_i' = a_i$, $b_i' = us'sb_i$. The inverse map is well-defined. The maps in both directions are obvious mutual inversions.

$\Spec(B_\ppp/\ppp B_\ppp) = \Spec(k(\ppp) \otimes_A B)$ 

\end{document}
